Compiler.thy
@@ -2,74 +2,124 @@ theory Compiler
   imports "01Source/AlgorithmicTypechecking" Printing "03Stack/StackConversion" 
 begin
 
-definition compile :: "nexpr \<Rightarrow> byte_code list" where
-  "compile = flatten_code \<circ> tco \<circ> encode \<circ> convert"
+primrec get_return :: "nat \<Rightarrow> nexpr \<Rightarrow> tco_return" where
+  "get_return d (NVar x) = TCOReturn d"
+| "get_return d (NConst k) = TCOReturn d"
+| "get_return d (NLam x t e) = TCOReturn d"
+| "get_return d (NApp e\<^sub>1 e\<^sub>2) = TCOJump d"
 
-primrec one_pass_r' :: "nat \<Rightarrow> nexpr \<Rightarrow> tco_return" where
-  "one_pass_r' d (NVar x) = TCOReturn d"
-| "one_pass_r' d (NConst k) = TCOReturn d"
-| "one_pass_r' d (NLam x t e) = TCOReturn d"
-| "one_pass_r' d (NApp e\<^sub>1 e\<^sub>2) = TCOJump d"
+primrec flatten_return :: "tco_return \<Rightarrow> byte_code" where 
+  "flatten_return (TCOReturn d) = BReturn d"
+| "flatten_return (TCOJump d) = BJump d"
 
-primrec one_pass_cd' :: "var list \<Rightarrow> nat \<Rightarrow> tco_code list \<Rightarrow> bool \<Rightarrow> nexpr \<Rightarrow> tco_code list" where
-  "one_pass_cd' \<Phi> d cd b (NVar x) = TCOLookup (the (idx_of \<Phi> x)) # cd"
-| "one_pass_cd' \<Phi> d cd b (NConst k) = TCOPushCon k # cd"
-| "one_pass_cd' \<Phi> d cd b (NLam x t e) = 
-    TCOPushLam (one_pass_cd' (insert_at 0 x \<Phi>) (Suc d) [] True e) (one_pass_r' (Suc d) e) d # cd"
-| "one_pass_cd' \<Phi> d cd b (NApp e\<^sub>1 e\<^sub>2) = 
-    one_pass_cd' \<Phi> d (one_pass_cd' \<Phi> d (if b then cd else TCOApply # cd) False e\<^sub>2) False e\<^sub>1"
+function xflatten_code' :: "nat \<Rightarrow> nat \<Rightarrow> byte_code list \<Rightarrow> tco_code list \<Rightarrow> 
+    byte_code list \<times> byte_code list \<times> nat" where
+  "xflatten_code' ofst sz acc [] = ([], acc, Suc (ofst + sz))"
+| "xflatten_code' ofst sz acc (TCOLookup x # cd) = 
+    xflatten_code' ofst (Suc sz) (BLookup x # acc) cd"
+| "xflatten_code' ofst sz acc (TCOPushCon k # cd) = 
+    xflatten_code' ofst (Suc sz) (BPushCon k # acc) cd"
+| "xflatten_code' ofst sz acc (TCOPushLam cd' r' d # cd) = (case xflatten_code' ofst 0 [] cd' of
+    (lib', cdb', sz') \<Rightarrow> (case xflatten_code' sz' (Suc sz) (BPushLam sz' d # acc) cd of
+      (lib, cdb, sz'') \<Rightarrow> (lib' @ flatten_return r' # cdb' @ lib, cdb, sz'')))"
+| "xflatten_code' ofst sz acc (TCOApply # cd) = xflatten_code' ofst (Suc sz) (BApply # acc) cd"
+  by pat_completeness auto
+termination
+  by (relation "measure (code_list_size \<circ> snd \<circ> snd \<circ> snd)") simp_all
 
-definition one_pass :: "nexpr \<Rightarrow> tco_code list \<times> tco_return" where
-  "one_pass e = (one_pass_cd' [] 0 [] True e, one_pass_r' 0 e)"
+primrec compile' :: "var list \<Rightarrow> nat \<Rightarrow> tco_code list \<Rightarrow> bool \<Rightarrow> nexpr \<Rightarrow> tco_code list" where
+  "compile' var_idxs depth acc tail_pos (NVar x) = TCOLookup (the (idx_of var_idxs x)) # acc"
+| "compile' var_idxs depth acc tail_pos (NConst k) = TCOPushCon k # acc"
+| "compile' var_idxs depth acc tail_pos (NLam x t e) = 
+    TCOPushLam (compile' (x # var_idxs) (Suc depth) [] True e) 
+      (get_return (Suc depth) e) depth # acc"
+| "compile' var_idxs depth acc tail_pos (NApp e\<^sub>1 e\<^sub>2) = 
+    compile' var_idxs depth 
+      (compile' var_idxs depth (if tail_pos then acc else TCOApply # acc) False e\<^sub>2) False e\<^sub>1"
 
-lemma [simp]: "one_pass_r' d e = tco_r d (encode' (convert' \<Phi> e) d' [])"
+primrec xflatten_code :: "tco_code list \<times> tco_return \<Rightarrow> byte_code list \<times> nat" where
+  "xflatten_code (cd, r) = (case xflatten_code' 0 0 [] cd of
+    (lib, cdb, sz) \<Rightarrow> (lib @ flatten_return r # cdb, sz))"
+
+definition compile :: "nexpr \<Rightarrow> tco_code list \<times> tco_return" where
+  "compile e = (compile' [] 0 [] True e, get_return 0 e)"
+
+lemma [simp]: "[flatten_return r] = flatten_code' lib [] r"
+  by (induction r) simp_all
+
+lemma flatten'_correctness [simp]: "sz = length acc \<Longrightarrow> 
+  xflatten_code' ofst sz acc cd = (lib, cdb, sz') \<Longrightarrow> 
+    sz' = ofst + code_list_size cd + sz \<and> 
+      lib @ flatten_return r # cdb = flatten_code' ofst cd r @ acc"
+proof (induction ofst sz acc cd arbitrary: lib cdb sz' r rule: xflatten_code'.induct)
+  case (4 ofst sz acc cd' r' d cd)
+  moreover obtain lib' cdb' sz'' where "xflatten_code' ofst 0 [] cd' = (lib', cdb', sz'')" 
+    by (cases "xflatten_code' ofst 0 [] cd'")
+  moreover obtain lib2 cdb2 sz2 where 
+    "xflatten_code' sz'' (Suc sz) (BPushLam sz'' d # acc) cd = (lib2, cdb2, sz2)" 
+      by (cases "xflatten_code' sz'' (Suc sz) (BPushLam sz'' d # acc) cd")
+  ultimately show ?case by force
+qed (auto split: prod.splits)
+
+lemma [simp]: "xflatten_code cdr = (flatten_code cdr, length (flatten_code cdr))"
+proof (cases cdr)
+  case (Pair cd r)
+  moreover obtain lib cdb sz where S :"xflatten_code' 0 0 [] cd = (lib, cdb, sz)" 
+    by (cases "xflatten_code' 0 0 [] cd") simp_all
+  moreover have "0 = length []" by simp
+  moreover with S have "sz = 0 + code_list_size cd + length [] \<and> 
+    lib @ flatten_return r # cdb = flatten_code' 0 cd r @ []" by (metis flatten'_correctness)
+  ultimately show ?thesis by simp
+qed
+
+lemma [simp]: "get_return d e = tco_r d (encode' (convert' \<Phi> e) d')"
 proof (induction e arbitrary: \<Phi> d)
   case (NApp e1 e2)
-  have "tco_r d ((encode' (convert' \<Phi> e1) d' [] @ encode' (convert' \<Phi> e2) d' []) @ [TApply]) = 
+  have "tco_r d ((encode' (convert' \<Phi> e1) d' @ encode' (convert' \<Phi> e2) d') @ [TApply]) = 
     tco_r d [TApply]" using tco_r_append by blast
   thus ?case by simp
 qed simp_all
 
-lemma one_pass_cd_correct [simp]: "cd' = tco_cd cd \<Longrightarrow> 
-  one_pass_cd' \<Phi> d cd' (cd = []) e = tco_cd (encode' (convert' \<Phi> e) d cd)"
+lemma compile_correct [simp]: "cd' = tco_cd cd \<Longrightarrow> 
+  compile' \<Phi> d cd' (cd = []) e = tco_cd (encode' (convert' \<Phi> e) d @ cd)"
 proof (induction e arbitrary: \<Phi> d cd cd')
   case (NLam x t e)
   moreover have "[] = tco_cd []" by simp
-  ultimately have "one_pass_cd' (insert_at 0 x \<Phi>) (Suc d) [] True e =
-    tco_cd (encode' (convert' (insert_at 0 x \<Phi>) e) (Suc d) [])" by (metis (full_types))
-  with NLam show ?case by simp
+  ultimately have "compile' (x # \<Phi>) (Suc d) [] True e =
+    tco_cd (encode' (convert' (x # \<Phi>) e) (Suc d) @ [])" by (metis (full_types))
+  with NLam show ?case by (cases \<Phi>) simp_all
 next
   case (NApp e1 e2)
   hence "(if cd = [] then cd' else TCOApply # cd') = tco_cd (TApply # cd)" 
     by (simp split: list.splits)
-  with NApp have "one_pass_cd' \<Phi> d (if cd = [] then cd' else TCOApply # cd') 
+  with NApp have "compile' \<Phi> d (if cd = [] then cd' else TCOApply # cd') 
     (TApply # cd = []) e2 = 
-      tco_cd (encode' (convert' \<Phi> e2) d (TApply # cd))" by blast
-  moreover from NApp have "one_pass_cd' \<Phi> d (tco_cd (encode' (convert' \<Phi> e2) d (TApply # cd))) 
-    (encode' (convert' \<Phi> e2) d (TApply # cd) = []) e1 = 
-      tco_cd (encode' (convert' \<Phi> e1) d (encode' (convert' \<Phi> e2) d (TApply # cd)))" by blast
+      tco_cd (encode' (convert' \<Phi> e2) d @ TApply # cd)" by blast
+  moreover from NApp have "compile' \<Phi> d (tco_cd (encode' (convert' \<Phi> e2) d @ TApply # cd)) 
+    ((encode' (convert' \<Phi> e2) d @ TApply # cd) = []) e1 = 
+      tco_cd (encode' (convert' \<Phi> e1) d @ encode' (convert' \<Phi> e2) d @ TApply # cd)" by blast
   ultimately show ?case by simp
 qed simp_all
 
-lemma [simp]: "one_pass = tco \<circ> encode \<circ> convert"
-proof (rule, unfold one_pass_def tco_def encode_def convert_def)
+lemma [simp]: "compile = tco \<circ> encode \<circ> convert"
+proof (rule, unfold compile_def tco_def encode_def convert_def)
   fix e
   have "[] = tco_cd []" by simp
-  hence "one_pass_cd' [] 0 [] ([] = []) e = tco_cd (encode' (convert' [] e) 0 [])" 
-    by (metis (full_types) one_pass_cd_correct)
-  thus "(one_pass_cd' [] 0 [] True e, one_pass_r' 0 e) =
-    ((\<lambda>cd. (tco_cd cd, tco_r 0 cd)) \<circ> (\<lambda>e. encode' e 0 []) \<circ> convert' []) e" by simp
+  hence "compile' [] 0 [] ([] = []) e = tco_cd (encode' (convert' [] e) 0 @ [])" 
+    by (metis (full_types) compile_correct)
+  thus "(compile' [] 0 [] True e, get_return 0 e) =
+    ((\<lambda>cd. (tco_cd cd, tco_r 0 cd)) \<circ> (\<lambda>e. encode' e 0) \<circ> convert' []) e" by simp
 qed
 
-lemma [simp]: "tco_cd (encode' e d acc) \<noteq> []"
-  by (induction e arbitrary: acc) simp_all
+lemma [simp]: "tco_cd (encode' e d) \<noteq> []"
+  by (induction e) simp_all
 
 lemma [simp]: "tco_cd (encode e) \<noteq> []"
   by (simp add: encode_def)
 
-theorem tc_terminationn: "typechecks e \<Longrightarrow> compile e = cd \<Longrightarrow> 
+theorem tc_terminationn: "typechecks e \<Longrightarrow> xflatten_code (compile e) = (cd, pc) \<Longrightarrow> 
   \<exists>v. valn v \<and> e \<Down> v \<and> 
-    (\<exists>h v\<^sub>f. iter (\<leadsto>\<^sub>f) (FS hempty [] [[length cd]] cd) (FS h [v\<^sub>f] [] cd) \<and> 
+    (\<exists>h v\<^sub>f. iter (\<leadsto>\<^sub>f) (FS hempty [] [[pc]] cd) (FS h [v\<^sub>f] [] cd) \<and> 
       print_hclosure (get_closure h v\<^sub>f) = print_nexpr v)"
 proof -
   assume "typechecks e"
@@ -94,28 +144,29 @@ proof -
     (tco_state (TS [encode_closure c] []))" by (metis iter_tco_eval)
   hence ET: "iter (\<leadsto>\<^sub>t\<^sub>c\<^sub>o) (TCOS [] [([], tco_cd (encode (convert e)), tco_r 0 (encode (convert e)))]) 
     (TCOS [tco_val (encode_closure c)] [])" by simp
-  assume "compile e = cd"
-  hence C: "flatten_code (tco (encode (convert e))) = cd" by (simp add: compile_def)
-  hence UB: "unflatten_state (BS [] [([], length cd)] cd) = 
+  assume "xflatten_code (compile e) = (cd, pc)"
+  hence C: "flatten_code (tco (encode (convert e))) = cd \<and> 
+    pc = length (flatten_code (tco (encode (convert e))))" by auto
+  hence UB: "unflatten_state (BS [] [([], pc)] cd) = 
     TCOS [] [([], tco_cd (encode (convert e)), tco_r 0 (encode (convert e)))]" 
       by (auto simp add: tco_def simp del: flatten_code.simps)
-  from C have "orderly_state (BS [] [([], length cd)] cd)" by auto
+  from C have "orderly_state (BS [] [([], pc)] cd)" by auto
   with ET UB obtain v\<^sub>b where EB: 
-    "iter (\<leadsto>\<^sub>b) (BS [] [([], length cd)] cd) (BS [v\<^sub>b] [] cd) \<and> 
+    "iter (\<leadsto>\<^sub>b) (BS [] [([], pc)] cd) (BS [v\<^sub>b] [] cd) \<and> 
       tco_val (encode_closure c) = unflatten_closure cd v\<^sub>b" 
     by (metis evalb_end byte_code_state.sel(3))
   hence "print_bclosure v\<^sub>b = print_tco_closure (tco_val (encode_closure c))" by simp
   with VC have VB: "print_bclosure v\<^sub>b = print_nexpr v\<^sub>n" by simp
-  from EB obtain \<Sigma>\<^sub>h' where EH: "iter (\<leadsto>\<^sub>h) (HS hempty [] [([], length cd)] cd) \<Sigma>\<^sub>h' \<and> 
+  from EB obtain \<Sigma>\<^sub>h' where EH: "iter (\<leadsto>\<^sub>h) (HS hempty [] [([], pc)] cd) \<Sigma>\<^sub>h' \<and> 
     BS [v\<^sub>b] [] cd = unheap \<Sigma>\<^sub>h'" by fastforce
   then obtain h\<^sub>h v\<^sub>h where SH: "\<Sigma>\<^sub>h' = HS h\<^sub>h [v\<^sub>h] [] cd \<and> v\<^sub>b = unheap_closure h\<^sub>h v\<^sub>h" 
     using unheap_empty by blast
   with VB have VH: "print_hclosure (hlookup h\<^sub>h v\<^sub>h) = print_nexpr v\<^sub>n" by simp
-  have HS: "heap_structured (HS hempty [] [([], length cd)] cd)" by simp
-  have FS: "flatten (HS hempty [] [([], length cd)] cd) = FS hempty [] [[length cd]] cd" by simp
+  have HS: "heap_structured (HS hempty [] [([], pc)] cd)" by simp
+  have FS: "flatten (HS hempty [] [([], pc)] cd) = FS hempty [] [[pc]] cd" by simp
   obtain h\<^sub>f mp where HC: "hsplay splay_closure h\<^sub>h = (h\<^sub>f, mp)" by fastforce
   with SH have "flatten \<Sigma>\<^sub>h' = FS h\<^sub>f [mp v\<^sub>h] [] cd" by simp
-  with EH FS HS have EF: "iter (\<leadsto>\<^sub>f) (FS hempty [] [[length cd]] cd) (FS h\<^sub>f [mp v\<^sub>h] [] cd)"
+  with EH FS HS have EF: "iter (\<leadsto>\<^sub>f) (FS hempty [] [[pc]] cd) (FS h\<^sub>f [mp v\<^sub>h] [] cd)"
     by (metis completef_iter)
   from EH have "heap_structured \<Sigma>\<^sub>h'" by fastforce
   with SH have "hcontains h\<^sub>h v\<^sub>h" by simp
@@ -126,7 +177,7 @@ proof -
 
 
 
-  from EF VF have "iter (\<leadsto>\<^sub>f) (FS hempty [] [[length cd]] cd) (FS h\<^sub>f [mp v\<^sub>h] [] cd) \<and> 
+  from EF VF have "iter (\<leadsto>\<^sub>f) (FS hempty [] [[pc]] cd) (FS h\<^sub>f [mp v\<^sub>h] [] cd) \<and> 
     print_hclosure (get_closure h\<^sub>f (mp v\<^sub>h)) = print_nexpr v\<^sub>n" by simp
   with EN VN show ?thesis by fastforce
 qed
